Answer:

L(O) = [O]

L(A) = [A] + merge L(L(O), [O]) = [A] + merge L([0], [0]) = [A, O] 同理 L(A) = [B,O] = [C,O]

L(K1) = [K1] + merge L(L(A), L(B), [A, B]) = [K1] + merge L([A, O], [B, O], [A, B]) = [K1, A] + merge L([O], [B, O], [B]) = [K1, A, B] + merge L([O], [O], [O]) = [K1, A, B, O]

L(K2) = [K2] + merge L(L(A), L(C), [A, C]) = [K2] + merge L([A, O], [C, O], [A, C]) = [K2, A] + merge L([O], [C, O], [C]) = [K2, A, C] + merge L([O], [O], [O]) = [K2, A, C, O]

L(Z) = [Z] + merge L(L(K1), L(K2), [K1, K2]) = [Z] + merge L([K1, A, B, O], [K2, A, C, O], [K1, K2]) = [Z, K1] + merge L([A, B, O], [K2, A, C, O], [K2]) = [Z, K1, K2] + merge L([A, B, O], [A, C, O]) = [Z, K1, K2, A] + merge L([B, O], [C,O]) = [Z, K1, K2, A, B] + merge L([O], [C, O]) = [Z, K1, K2, A, B, C] + merge L([O], [O]) = [Z, K1, K2, A, B, C, O]